{
 "cells": [
  {
   "cell_type": "markdown",
   "metadata": {},
   "source": [
    "# Finding Solution for Inhomogeneous ODE\n",
    "\n",
    "$$y'' + Ay' + By = f(x)$$\n",
    "\n",
    "Find a particular solution $y_p$. Then the general solution is $y = y_p + c_1y_1 + c_2y_2$\n",
    "\n",
    "Important $f(x):$ $e^{ax} (a < 0)$, $\\sin \\omega x, \\cos\\omega x$, $e^{ax} \\sin \\omega x, e^{ax} \\cos \\omega x$\n",
    "\n",
    "They are all special cases of $e^{(a + ib)x}$\n",
    "\n",
    "$e^{(a + ib)x}$ can be simplied as $e^{\\alpha x}$ with $\\alpha$ complex number and this is going to be our input\n",
    "\n",
    "Think of the left hand side as polynomial operator\n",
    "\n",
    "$$(D^2 + AD + B)y = f(x)$$\n",
    "\n",
    "with $p(D) = D^2 + AD + B$\n",
    "\n",
    "An important equation that we will be using. Substitution rule\n",
    "\n",
    "$$p(D) e^{\\alpha x} = p(\\alpha) e^{\\alpha x}$$\n",
    "\n",
    "Prove: \n",
    "$$\\begin{align}(D^2 + AD + B)e^{\\alpha x} & = D^2 e^{\\alpha x} + ADe^{\\alpha x} + Be^{\\alpha x} \\\\\n",
    "& = \\alpha^2 e^{\\alpha x} + A\\alpha e^{\\alpha x} + Be^{\\alpha x} \\\\\n",
    "& = e^{\\alpha x}(\\alpha^2 + A\\alpha + B) \\\\\n",
    "& = p(\\alpha) e^{\\alpha x}\n",
    "\\end{align}$$"
   ]
  },
  {
   "cell_type": "markdown",
   "metadata": {},
   "source": [
    "## Exponential Input Theorem\n",
    "\n",
    "$$y_p = \\frac{e^{\\alpha x}}{p(\\alpha)}$$\n",
    "\n",
    "Prove if I apply $p(D)$ to $y_p$, do I get $e^{\\alpha x}$: \n",
    "\n",
    "$$p(D)y_p = e^{\\alpha x}$$\n",
    "\n",
    "$$p(D) \\frac{e^{\\alpha x}}{p(\\alpha)} = \\frac{p(\\alpha)e^{\\alpha x}}{p(\\alpha)} = e^{\\alpha x}$$\n",
    "\n",
    "If $p(\\alpha) = 0$, this won't work. We will cater it later, for the time being assume $p(\\alpha) \\neq 0$\n",
    "\n",
    "\n",
    "### Example\n",
    "\n",
    "Find the particular solution for $$y'' - y' + 2y = 10e^{-x}\\sin x$$\n",
    "\n",
    "Start with polynomial operator and complexify the input. $e^{-x}\\sin x$ is the imaginary part of $e^{(-1 + i)x}$\n",
    "\n",
    "$$(D^2 - D + 2)\\tilde y = 10e^{(-1 + i)x}$$\n",
    "\n",
    "$\\tilde y$ to indicate the solution we get is not the solution for original equation. From the theorem, we get\n",
    "\n",
    "$$\\tilde y_p = \\frac{10e^{(-1 + i)x}}{(-1 + i)^2 - (-1 + i) + 2}$$\n",
    "\n",
    "$$\\tilde y_p = \\frac{10e^{(-1 + i)x}}{3 - 3i} = \\frac{10}{3}\\frac{i + 1}{2}e^{-x}(\\cos x + i\\sin x)$$\n",
    "\n",
    "$$\\begin{align}\n",
    "y_p & = Im(\\tilde y_p) \\\\\n",
    "& = \\frac53 e^{-x} (\\cos x + \\sin x) \\\\\n",
    "& = \\frac53 e^{-x} \\sqrt{2} \\cos(x - \\frac{\\pi}{4})\n",
    "\\end{align}$$\n",
    "\n",
    "\n",
    "### Case $p(a) = 0$\n",
    "\n",
    "Change variable $\\alpha$ to $a$ for easier writing.\n",
    "\n",
    "Exponential-shift rule $$p(D)e^{ax} u(x) = e^{ax} p(D + a) u(x)$$\n",
    "\n",
    "This rule is just direct consequence of differentiation product rule\n",
    "\n",
    "To prove the rule, just starts with simple $p(D) = D$\n",
    "\n",
    "$$\\begin{align}\n",
    "De^{ax}u & = e^{ax}Du + ae^{ax}u \\\\\n",
    "& = e^{ax}(D + a)u\n",
    "\\end{align}$$\n",
    "\n",
    "If this is true also for $D^2$?\n",
    "\n",
    "$$\\begin{align}\n",
    "D^2e^{ax}u & = D(De^{ax}u) \\\\\n",
    "& = D(e^{ax}(D + a)u \\\\\n",
    "& = e^{ax}(D + a)(D + a)u \\\\\n",
    "& = e^{ax}(D + a)^2 u\n",
    "\\end{align}$$\n",
    "\n",
    "We can see that the process can be generalized to n-th derivative by induction\n",
    "\n"
   ]
  },
  {
   "cell_type": "markdown",
   "metadata": {},
   "source": [
    "Back to the form\n",
    "\n",
    "$$(D^2 + AD + B)y = e^{ax}$$\n",
    "\n",
    "with $a$ is allowed to be complex and $p(x) = 0$. \n",
    "\n",
    "$$y_p = \\frac{xe^{ax}}{p'(a)}$$\n",
    "\n",
    "$a$ is a simple root of $p(D)$. Is $p'(a)$ guaranteed no zero? Yes\n",
    "\n",
    "Proof: if $a$ is simple root case, it can be factored out, so\n",
    "\n",
    "$$p(D) = (D - b)(D - a), b \\neq a$$\n",
    "\n",
    "By product rule\n",
    "\n",
    "$$p'(D) = (D - a) + (D - b)$$\n",
    "\n",
    "$$p'(a) = a - b$$\n",
    "\n",
    "This proves that if $a$ is simple, $p'(a)$ is guaranteed not to be zero\n",
    "\n",
    "What if $a$ is double root?\n",
    "\n",
    "In that case, $$y_p = \\frac{x^2 e^{ax}}{p''(a)}$$\n",
    "\n",
    "Things go on for higher root\n",
    "\n",
    "\n",
    "### Now propose $y_p = \\frac{e^{ax}x}{p'(a)}$ is the solution\n",
    "\n",
    "We need to check if the following statement is true\n",
    "\n",
    "$$p(D)y_p = p(D) \\frac{e^{ax}x}{p'(a)} = e^{ax}$$\n",
    "\n",
    "By exponential-shift rule\n",
    "\n",
    "$$e^{ax}\\frac{(D + a - b)Dx}{p'(a)} = e^{ax}\\frac{a - b}{a - b} = e^{ax}$$"
   ]
  },
  {
   "cell_type": "markdown",
   "metadata": {},
   "source": [
    "### Example\n",
    "\n",
    "$$y'' - 3y' + 2y = e^x$$\n",
    "\n",
    "$a = 1$ is simple root of $D^2 - 3D + 2$. If this is double root, ODE won't look like that\n",
    "\n",
    "$$p'(D) = 2D - 3 \\implies p'(1) = -1$$\n",
    "\n",
    "$$y_p = \\frac{xe^x}{-1} = -xe^x$$\n"
   ]
  },
  {
   "cell_type": "code",
   "execution_count": null,
   "metadata": {},
   "outputs": [],
   "source": []
  }
 ],
 "metadata": {
  "kernelspec": {
   "display_name": "Julia 1.5.0",
   "language": "julia",
   "name": "julia-1.5"
  },
  "language_info": {
   "file_extension": ".jl",
   "mimetype": "application/julia",
   "name": "julia",
   "version": "1.5.0"
  }
 },
 "nbformat": 4,
 "nbformat_minor": 4
}
