{
 "cells": [
  {
   "cell_type": "markdown",
   "metadata": {},
   "source": [
    "# First Order Linear Equation\n",
    "\n",
    "$$a(x)y' + b(x)y = c(x)$$\n",
    "\n",
    "x can be appeared much arbitrary in the equation compare to y which is somewhat limited. It is linear in y and y'. Linear like in the equation $ay_1 + by_2 = c$. It is homogenous if c = 0\n",
    "\n",
    "Standard Linear Form: $$y' + p(x)y = q(x)$$\n",
    "\n",
    "($y' = p(x)y + q(x)$ is other standard 1st order form which will not be used in this course)\n",
    "\n",
    "What so important about this equation?\n",
    "1. It can be always be solved\n",
    "2. It arised in many models\n",
    "\n",
    "## Models\n",
    "1. Temperature-concentration model\n",
    "2. Mixing model\n",
    "3. Decay, bank, some motion problems\n",
    "\n",
    "## Temperature-concentration model\n",
    "\n",
    "### Conduction\n",
    "\n",
    "Suppose a vacuum inside a water tank and a box inside the vacuum. T for temperature inside the box, $T_e$ is the temperature of the water. Temperature of water goes into the temperature of the box only by conduction.\n",
    "\n",
    "Newton law of cooling. $T$ is the temperature inside, $T_e$ is the temperature outside which is bigger and $t$ is the time. We want to write it so that $k > 0$ where k is the conductivity.\n",
    "\n",
    "$$\\frac{dT}{dt} = k(T_e - T)$$\n",
    "\n",
    "Initial condition $T(0) = T_0$\n",
    "\n",
    "### Diffusion\n",
    "\n",
    "$C =$ salt concentraion inside. $C_e =$ salt concentration outide. The salt diffuse from outside into inside (membrane wall)\n",
    "\n",
    "$$\\frac{dC}{dt} = k(C_e - C)$$\n",
    "\n",
    "We expect salt to flow in, so $k > 0$\n",
    "\n",
    "These two differential equation models the physical situation of conduction and diffusion.\n",
    "\n"
   ]
  },
  {
   "cell_type": "markdown",
   "metadata": {},
   "source": [
    "First converts it to standard linear form\n",
    "\n",
    "$$T' + kT = kT_e$$\n",
    "\n",
    "$T_e$ can be a general function of $T$. Here $k$ is constant, but this is not necessary, it can be varying over time.\n",
    "\n",
    "Back to the standard form: $$y' + p(x)y = q(x)$$\n",
    "\n",
    "We can solve it by integrating factor: $u(x)$. Multiply the equation with this factor\n",
    "\n",
    "$$uy' + puy + qu$$\n",
    "\n",
    "So that we can write the equation as follow\n",
    "\n",
    "$$(uy)' = qu$$\n",
    "\n",
    "Then we can solve it. In order to achive this, u' has to be equal to pu $$u' = pu$$\n",
    "\n",
    "Integrate with separation variable\n",
    "\n",
    "$$ \\int \\frac{u'}{u}\\ du = \\int p(x)\\ dx$$\n",
    "$$ln\\ u = \\int p(x)\\ dx$$\n",
    "$$u = e^{\\int p\\ dx}$$\n",
    "\n",
    "This is called the integrating factor. (No arbitrary constant, since only one $u$ you needed)\n",
    "\n",
    "## Method\n",
    "\n",
    "1. Put it in standard linear form $y' + py = q$\n",
    "2. Calculate integrating factor $e^{\\int p\\ dx}$\n",
    "3. Multiply both sides by $e^{\\int p\\ dx}$\n",
    "4. Integrate"
   ]
  },
  {
   "cell_type": "markdown",
   "metadata": {},
   "source": [
    "## Example\n",
    "\n",
    "$$xy' - y = x^3$$\n",
    "\n",
    "Put it in standard form\n",
    "\n",
    "$$y' - \\frac{1}{x}y = x^2$$\n",
    "\n",
    "$\\int 1/x\\ dx = -ln\\ x$, hence integrating factor, $$e^{-ln\\ x} = (e^{ln\\ x})^{-1} = \\frac1x$$\n",
    "\n",
    "Multiply both sides by integrating factor\n",
    "\n",
    "$$\\frac{1}{x}y' - \\frac{1}{x^2}y = x$$\n",
    "\n",
    "$$(\\frac1x y)' = x$$\n",
    "\n",
    "Do the integration\n",
    "\n",
    "$$\\frac{y}{x} = \\frac{x^2}{2} + C$$\n",
    "\n",
    "Solution is\n",
    "\n",
    "$$y = \\frac{x^3}{2} + Cx$$"
   ]
  },
  {
   "cell_type": "markdown",
   "metadata": {},
   "source": [
    "## Example\n",
    "\n",
    "$$(1 + \\cos x)y' - (\\sin x)y = 2x$$\n",
    "\n",
    "$$y' - \\frac{\\sin x}{1 + \\cos x}y = \\frac{2x}{1 + \\cos x}$$\n",
    "\n",
    "Look for integrating factor: $$-\\int \\frac{\\sin x}{1 + \\cos x}\\ dx = ln\\ (1 + \\cos x)$$\n",
    "\n",
    "Integrating factor: $$e^{ln(1 + \\cos x)} = 1 + \\cos x$$\n",
    "\n",
    "Multiplying both side with I.F.\n",
    "\n",
    "$$(1 + \\cos x)^2y' - y\\sin x = 2x$$\n",
    "\n",
    "$$[(1 + \\cos x)y]' = 2x$$\n",
    "\n",
    "$$(1 + \\cos x)y = x^2 + C$$\n",
    "\n",
    "$$y = \\frac{x^2 + C}{1 + \\cos x}$$\n",
    "\n",
    "Suppose initial condition $y(0) = 1$, then we can get $C$\n",
    "\n",
    "$$1 = \\frac{C}{2}$$\n",
    "\n",
    "$$C = 2$$\n",
    "\n",
    "$$y = \\frac{x^2 + 2}{1 + \\cos x}$$"
   ]
  },
  {
   "cell_type": "markdown",
   "metadata": {},
   "source": [
    "## Linear with $k$ constant\n",
    "\n",
    "$$\\frac{dT}{dt} + kT = kT_e$$\n",
    "\n",
    "I.F. $e^{kt}$, multiplied by $e^{kt}$\n",
    "\n",
    "$$(e^{kt}T)' = kT_e e^{kt}$$\n",
    "\n",
    "$T_e$ is the function of time t\n",
    "\n",
    "Integrate: $$e^{kt}T = \\int kT_e(t)e^{kt} + C$$\n",
    "\n",
    "$$T = e^{-kt}\\int kT_e(t)e^{kt}\\ dt + Ce^{-kt}$$\n",
    "\n",
    "Initial condition, $T(0) = T_0$\n",
    "\n",
    "$$T = e^{-kt}\\int_0^t kT_e(t_1)e^{kt_1}\\ dt_1 + Ce^{-kt}$$\n",
    "\n",
    "At $t = 0$, the integral term disappear, $C = T_0$.\n",
    "\n",
    "As $t \\to \\infty$, $Ce^{-kt} \\to 0$ provided $k > 0$\n",
    "\n",
    "Hence the equation can be seen as $$T = \\text{steady state solution} + \\text{transient solution}$$"
   ]
  },
  {
   "cell_type": "code",
   "execution_count": null,
   "metadata": {},
   "outputs": [],
   "source": []
  },
  {
   "cell_type": "code",
   "execution_count": null,
   "metadata": {},
   "outputs": [],
   "source": []
  }
 ],
 "metadata": {
  "kernelspec": {
   "display_name": "Julia 1.5.0",
   "language": "julia",
   "name": "julia-1.5"
  },
  "language_info": {
   "file_extension": ".jl",
   "mimetype": "application/julia",
   "name": "julia",
   "version": "1.5.0"
  }
 },
 "nbformat": 4,
 "nbformat_minor": 4
}
