{
 "cells": [
  {
   "cell_type": "markdown",
   "metadata": {},
   "source": [
    "# Oscillations\n",
    "\n",
    "$$y'' + by' + ky = 0$$\n",
    "\n",
    "try $y = e^{rt}$, we can see root satisfy $$r^2 + br + k = 0$$\n",
    "\n",
    "Oscillation correspond to complex root of $r^2 + br + k = 0$\n",
    "\n",
    "$$r = a \\pm bi$$\n",
    "\n",
    "Last lecture took $r = a + bi$, leads to solution $e^{(a + ib)t}$. We separate the exponential into real and imaginary part. Both of those give solution $y_1 = e^{at}\\cos bt, y_2 = e^{at}\\sin bt$\n",
    "\n",
    "We need real solutions, because those equations are from real quantities. \n",
    "\n",
    "How about $r = a - bi$? That will give us \n",
    "\n",
    "$$y_1 = e^{at}\\cos(-bt) =  e^{at}\\cos bt$$\n",
    "$$y_2 = e^{at}\\sin (-bt) = -e^{at}\\sin bt$$\n",
    "\n",
    "The general solution is $y = c_1y_1 + c_2y_2$, so that will change the sign of $c_2$ but doesn't give any new solution\n",
    "\n",
    "\n",
    "General Solution\n",
    "\n",
    "$$y = c_1 e^{(a + bi)t} + c_2 e^{(a - bi)t}$$\n",
    "\n",
    "We are only interested in real solution, but above is a complex function. $c_1, c_2$ are also allowed to be complex. How do I get real solution from complex function?\n",
    "\n",
    "What are real solution? Let say the solution is $u + iv$\n",
    "\n",
    "First way, substitute $c_1, c_2$ to be complex numbers, expand the complex exponential, collect the terms and equal the imaginary part to zero and see what it looks like. $(v = 0)$\n",
    "\n",
    "Second way, change i to -i, see if stays the same. If after changing, the expression doesn't change, v must be zero.\n",
    "\n",
    "Starts from here, $$y = c_1 e^{(a + bi)t} + c_2 e^{(a - bi)t}$$\n",
    "\n",
    "Change $i$ to $-i$, and $c$ to its complex conjugate \n",
    "\n",
    "$$\\overline y = \\overline c_1 e^{(a - bi)t} + \\overline c_2 e^{(a + bi)t}$$\n",
    "\n",
    "We want these two equations to be the same. That happen when \n",
    "\n",
    "$$c_2 = \\overline c_1, \\overline c_2 = c_1$$\n",
    "\n",
    "Complex conjugate of a complex conjugate get back the same thing. So above is only one equation. Substitute $c_1 = c + id$\n",
    "\n",
    "$$y = (c + id) e^{(a + bi)t} + (c - id) e^{(a - bi)t}$$\n",
    "\n",
    "Many scientists and engineers write the solution this way.\n",
    "\n"
   ]
  },
  {
   "cell_type": "markdown",
   "metadata": {},
   "source": [
    "We can write the above form into sine and cosine\n",
    "\n",
    "$$y = e^{at}[c (e^{bit} + e^{-ibt}) + id (e^{ibt} - e{-ibt})]$$\n",
    "\n",
    "From Euler,\n",
    "$$\\cos a = \\frac{e^{ia} + e^{-ia}}{2}$$\n",
    "$$\\sin a = \\frac{e^{ia} - e^{-ia}}{2i}$$\n",
    "\n",
    "$$y = e^{at}[c (2\\cos bt) + id (2i\\sin bt)]$$\n",
    "\n",
    "$$y = e^{at}[2c\\cos bt - 2d\\sin bt]$$"
   ]
  },
  {
   "cell_type": "markdown",
   "metadata": {},
   "source": [
    "## Back to this form\n",
    "\n",
    "$$y'' + \\frac{c}{m}y' + \\frac{k}{m}y = 0$$\n",
    "\n",
    "Write this in this form. So that later the equation can be written nicer.\n",
    "\n",
    "$$y'' + 2py' + \\omega_0^2y = 0$$\n",
    "\n",
    "Oscillations (only happen when the equation has copmlex roots)\n",
    "\n",
    "$$r^2 + 2pr + \\omega_0^2 = 0$$\n",
    "\n",
    "$$r = -p \\pm \\sqrt{p^2 - \\omega_0^2}$$\n",
    "\n",
    "If $p = 0$, the equation becomes $y'' + \\omega_0^2 y = 0$. This is undamped case. The solutions are pure oscillation and $\\omega_0$ is the circular frequency of the solutions. Because $r = \\pm i\\omega_0$ ($a = 0, b = \\omega_0$)\n",
    "\n",
    "$$y = c_1 \\cos \\omega_0t + c_2 \\sin\\omega_0t = A\\cos(\\omega_0t - \\phi)$$\n",
    "\n",
    "\n",
    "\n",
    "### Damped Case\n",
    "\n",
    "If $p^2 - \\omega_0^2 < 0 \\implies p < \\omega_0$, get oscillations. In another words, half the damping less than circular frequency.\n",
    "\n",
    "Spacing between t-axis intersection is half \"period\", or $\\pi/\\omega_1$. $\\omega_1$ is pseudo-frequency. \n",
    "\n",
    "If damping goes up, $\\omega_1$ goes down. We can see from the equation below\n",
    "\n",
    "$$r = -p \\pm \\sqrt{-(\\omega_0^2 - p^2)} = -p \\pm \\sqrt{-\\omega_1^2}$$\n",
    "\n",
    "Solution: $$\\begin{align}y & = e^{-pt}(c_1\\cos \\omega_1t + c_2\\sin\\omega_1t) \\\\\n",
    "& = e^{-pt} A \\cos(\\omega_1t - \\phi)\n",
    "\\end{align}$$\n",
    "\n",
    "If the function cross t-axis at $t_1$, it crosses next time at $t_2$, hence\n",
    "\n",
    "$$t_2 = t_1 + \\frac{2\\pi}{\\omega_1}$$\n",
    "\n",
    "At first cross t-axis: $$\\omega_1 t_1 - \\phi = \\frac{\\pi}{2}$$\n",
    "\n",
    "At second cross t-axis: $$\\omega_1 t_2 - \\phi = \\omega_1(t_1 + \\frac{2\\pi}{\\omega_1}) - \\phi = \\frac{\\pi}{2} + 2\\pi$$\n",
    "\n",
    "Hence $\\omega_1$ is called pseudo-frequency\n",
    "\n",
    "Let analyze what depends on what from this equation\n",
    "\n",
    "$$y = e^{-pt} A \\cos(\\omega_1t - \\phi)$$\n",
    "\n",
    "$p$ - damping constant depends on ODE, $c/2m$. This tells us how much it is coming down\n",
    "\n",
    "$\\omega_1$ - depends on ODE, $\\omega_1^2 = \\omega_0^2 - p^2$. This is a triangle with $\\omega_0$ is the hypotenuse. So it depends on damping and spring constant.\n",
    "\n",
    "$\\phi$ - Phase lag depends on initial condition\n",
    "\n",
    "$A$ - Amplitude depends on initial condition\n"
   ]
  },
  {
   "cell_type": "code",
   "execution_count": null,
   "metadata": {},
   "outputs": [],
   "source": []
  }
 ],
 "metadata": {
  "kernelspec": {
   "display_name": "Julia 1.5.0",
   "language": "julia",
   "name": "julia-1.5"
  },
  "language_info": {
   "file_extension": ".jl",
   "mimetype": "application/julia",
   "name": "julia",
   "version": "1.5.0"
  }
 },
 "nbformat": 4,
 "nbformat_minor": 4
}
